working on awalk, need to fix inv

checker-isa19/shortest_path_neg_checker.c
@@ -166,16 +166,15 @@ int awalk(Graph *g, Cycle *C) {
     // u \in verts G
     if (C->start >= vertex_cnt(g)) return 0;
 
-    for(unsigned int z = 0; z < C->length - 1; z++) {
+    for(unsigned int z = 0; z < C->length; z++) {
         if(C->path[z] >= edge_cnt(g)) return 0;
         if(z != C->length - 1) {
             if(C->path[z+1] >= edge_cnt(g)) return 0;
             if(arcs(g, C->path[z]).second != arcs(g, C->path[z+1]).first) return 0;
         }
-        else {
-            if(arcs(g, C->path[z]).second != C->start) return 0;
-        }
     }
+
+    if(arcs(g, C->path[C->length - 1]).second != C->start) return 0;
 
     return 1;
 }
